rust/implementation/openssl3_impl/tunnel/context.rs
@@ -80,6 +80,7 @@ impl std::fmt::Debug for SslContext {
 }
 
 #[hax_lib::opaque]
+#[hax_lib::attributes]
 impl SslContext {
     /// Disables session caching on a SSL context.
     fn disable_session_cache_mode(&self) {
@@ -671,12 +672,6 @@ fn get_verify_mode_from_mode_and_x509_verifier(
 /// A boxed and pinned tunnel.
 pub(crate) type PinnedTunnel<'a> = Pin<Box<Tunnel<'a>>>;
 
-fn hax_try_from<'a> (
-    ctx: &'a crate::Context,
-    configuration: &pb_api::Configuration,
-) -> Result<Context<'a>> {
-    Context::try_from(ctx, configuration)
-}
 
 impl<'a> Context<'a> {
     /// Instantiates a new [`Context`] from a [protobuf configuration](`pb_api::Configuration`)
