proofs/fstar/extraction/Sandwich.Support.Pimpl.fst
@@ -7,10 +7,10 @@ open FStar.Mul
 assume
 val t_Pimpl': v_T: Type0 -> eqtype
 
-let t_Pimpl = t_Pimpl'
+let t_Pimpl (v_T: Type0) = t_Pimpl' v_T
 
 /// Returns a copy of the [`NonNull`] pointer.
 assume
 val impl_2__as_nonnull': #v_T: Type0 -> self: t_Pimpl v_T -> Core.Ptr.Non_null.t_NonNull v_T
 
-let impl_2__as_nonnull = impl_2__as_nonnull'
+let impl_2__as_nonnull (#v_T: Type0) = impl_2__as_nonnull' #v_T
